updating to new jasmin and easycrypt

proofs/eclib/bindings.ec
@@ -1,122 +1,45 @@
 require import AllCore List IntDiv QFABV.
 
 from Jasmin require import JModel_x86.
-from JazzEC require import Array256 Array640 Array320.
+from JazzEC require import Array4 Array5 Array6 Array7 Array8 Array9 Array16 Array24 Array25 Array32 Array48 Array128 Array160 Array256 Array384 Array768 Array960 Array1088 Array1024 Array1152 Array1408 Array1536 WArray1568 Array1410 Array1 Array2 Array640.
+from JazzEC require import WArray16 WArray32 WArray128 WArray160 WArray512 WArray960 WArray2048 WArray1536 Array1568 WArray1410 WArray384 WArray1088.
 
 import BitEncoding BS2Int BitChunking.
 
 require import JWord_extra.
 
-
-(*[size_flatten] (for uniform inner lists) *)
-lemma size_flatten' ['a] sz (ss: 'a list list):
- (forall x, x\in ss => size x = sz) =>
- size (flatten ss) = sz*size ss.
-proof.
-move=> H; rewrite size_flatten.
-rewrite StdBigop.Bigint.sumzE.
-rewrite StdBigop.Bigint.BIA.big_map.
-rewrite -(StdBigop.Bigint.BIA.eq_big_seq (fun _ => sz)) /=.
- by move=> x Hx; rewrite /(\o) /= H.
-by rewrite StdBigop.Bigint.big_constz count_predT.
-qed.
-
-lemma flatten_ctt_inj ['a] (n : int) (s s' : 'a list list):
-     0 < n =>
-     (forall (x : 'a list), x \in s => size x = n) =>
-     (forall (x : 'a list), x \in s' => size x = n) =>
-     flatten s = flatten s' <=> s = s'.
-move=> Hn H1 H2; split; last by auto.
-move => Hf.
-have ? : size s = size s'.
-+ have ? := size_flatten_ctt n s _;1:smt().
-  have ? := size_flatten_ctt n s' _;1:smt().
-  have ? : n * size s' = n * size s by smt().
-  by smt().
-apply (eq_from_nth []); 1:smt().
-move => i ib.
-apply (eq_from_nth witness);1:smt(mem_nth).
-move => ii iib.
-have -> : nth witness (nth [] s i) ii  = nth witness (flatten s) (i * n + ii) by rewrite (nth_flatten witness n);smt(@List).
-have -> : nth witness (nth [] s' i) ii  = nth witness (flatten s') (i * n + ii) by rewrite (nth_flatten witness n);smt(@List).
-by smt().
-qed.
-
-
-(* ----------- BEGIN BOOL BINDINGS ---------- *)
-op bool2bits (b : bool) : bool list = [b].
-op bits2bool (b: bool list) : bool = List.nth false b 0.
-
-op i2b (i : int) = (i %% 2 <> 0).
-op b2si (b: bool) = 0.
-
-bind bitstring bool2bits bits2bool b2i b2si i2b bool 1.
-realize size_tolist by auto.
-realize tolistP by auto.
-realize oflistP by rewrite /bool2bits /bits2bool;smt(size_eq1).
-realize ofintP by rewrite /bits2bool /int2bs => i; rewrite (nth_mkseq false) //. 
-realize touintP by rewrite /bool2bits /= => bv; rewrite bs2int_cons bs2int_nil /=. 
-realize tosintP by move => bv => //. 
-
-bind op bool (/\) "and".
-realize bvandP by move=> bv1 bv2; rewrite /bool2bits /#.
+require import Abs_bindings.
 
 
 (* ----------- BEGIN W4 BINDINGS ---------- *)
-
 theory W4.
 abbrev [-printing] size = 4.
 clone include BitWordSH with op size <- size
-rename "_XX" as "_4"
 proof gt0_size by done,
 size_le_256 by done.
 
 end W4. export W4 W4.ALU W4.SHIFT.
 
-bind bitstring W4.w2bits W4.bits2w W4.to_uint W4.to_sint W4.of_int W4.t 4.
-realize size_tolist by auto.
-realize tolistP by auto.
-realize oflistP by smt(W4.bits2wK). 
-realize ofintP by move => *;rewrite /of_int int2bs_mod.
-realize tosintP. move => bv /=;rewrite /to_sint /smod /= /BVA_Top_W4_t.msb.
-have -> /=: nth false (w2bits bv) (4 - 1) = 2 ^ (4 - 1) <= to_uint bv; last by smt().
-rewrite /to_uint. 
-rewrite -{2}(cat_take_drop 3 (w2bits bv)).
-rewrite bs2int_cat size_take 1:// W4.size_w2bits /=.
-rewrite -bs2int_div 1:// /= get_to_uint /=.
-rewrite -bs2int_mod 1:// /= /to_uint.
-by smt(bs2int_range mem_range W4.size_w2bits pow2_4).
-qed.
-realize touintP by smt().
+clone import JCircuits as JC4 with
+op size <- 4,
+theory W <- W4
+rename "_XX" as "_4".
 
 (* ----------- BEGIN W5 BINDINGS ---------- *)
-
 theory W5.
 abbrev [-printing] size = 5.
 clone include BitWordSH with op size <- size
-rename "_XX" as "_5"
 proof gt0_size by done,
 size_le_256 by done.
 
 end W5. export W5 W5.ALU W5.SHIFT.
 
-bind bitstring W5.w2bits W5.bits2w W5.to_uint W5.to_sint W5.of_int W5.t 5.
-realize size_tolist by auto.
-realize tolistP by auto.
-realize oflistP by smt(W5.bits2wK). 
-realize ofintP by move => *;rewrite /of_int int2bs_mod.
-realize tosintP. move => bv /=;rewrite /to_sint /smod /= /BVA_Top_W5_t.msb.
-have -> /=: nth false (w2bits bv) (5 - 1) = 2 ^ (5 - 1) <= to_uint bv; last by smt().
-rewrite /to_uint. 
-rewrite -{2}(cat_take_drop 4 (w2bits bv)).
-rewrite bs2int_cat size_take 1:// W5.size_w2bits /=.
-rewrite -bs2int_div 1:// /= get_to_uint /=.
-rewrite -bs2int_mod 1:// /= /to_uint.
-by smt(bs2int_range mem_range W5.size_w2bits pow2_5).
-qed.
-realize touintP by smt().
+clone import JCircuits as JC5 with
+op size <- 5,
+theory W <- W5
+rename "_XX" as "_5".
 
-(* ----------- BEGIN W8 BINDINGS ---------- *)
+  (* ----------- BEGIN W8 BINDINGS ---------- *)
 bind bitstring W8.w2bits W8.bits2w W8.to_uint W8.to_sint W8.of_int W8.t 8.
 realize size_tolist by auto.
 realize tolistP by auto.
@@ -132,12 +55,14 @@ rewrite -bs2int_mod 1:// /= /to_uint.
 by smt(bs2int_range mem_range W8.size_w2bits pow2_8).
 qed.
 realize touintP by smt().
-
+realize gt0_size by done.
 
 (* -------------------------------------------------------------------- *)
 bind op [W8.t & bool] W8."_.[_]" "get".
 
 realize bvgetP by done.
+realize le_size by done.
+realize eq1_size by done.
 
 (* -------------------------------------------------------------------- *)
 bind op W8.t W8.andw "and".
@@ -164,6 +89,9 @@ move => i ib;rewrite !W8.get_w2bits orwE.
 rewrite (nth_map (false,false) false) /=; 1: by smt(size_map size_zip W8.size_w2bits).  
 rewrite !(nth_zip false false) //=;congr; rewrite -W8.get_w2bits.
 qed.
+
+bind op [W8.t & W8.t] W8.(`>>`) "shrs".
+realize bvshrsP by move => bv1 bv2; rewrite /(`>>`) to_uint_shr; 1:smt(W8.to_uint_cmp).
 
 op srl_8 (w1 w2 : W8.t) : W8.t =
   w1 `>>>` W8.to_uint w2.
@@ -212,6 +140,29 @@ have ? : 2^10 = 1024 by rewrite /=.
 by smt(bs2int_range mem_range W10.size_w2bits).
 qed.
 realize touintP by smt().
+realize gt0_size by done.      
+
+bind op [W10.t & bool] W10."_.[_]" "get".
+realize le_size by auto.
+realize eq1_size by auto.
+realize bvgetP by auto.
+
+bind op [bool & W10.t] W10.init "init".
+realize size_1 by auto.
+realize bvinitP.
+move => f.  apply (eq_from_nth false).
++ rewrite size_w2bits (size_flatten' 1). 
+  move => x; rewrite mkseqP /= => Hx;elim Hx.
+  rewrite /bool2bits => /#.
+  rewrite size_mkseq /#.
+
+move => i; rewrite size_w2bits => ?.
+rewrite get_w2bits (nth_flatten false 1).
++ rewrite allP.
+  move => x; rewrite mkseqP /= => Hx;elim Hx.
+  rewrite /bool2bits => /#.
+by rewrite nth_mkseq 1:/# /= /bool2bits initiE 1:/# /=. 
+qed.
 
 (* ----------- BEGIN W10 BINDINGS -----------*)
 
@@ -240,6 +191,30 @@ have ? : 2^11 = 2048 by rewrite /=.
 by smt(bs2int_range mem_range W11.size_w2bits).
 qed.
 realize touintP by smt().
+realize gt0_size by done.
+
+
+bind op [W11.t & bool] W11."_.[_]" "get".
+realize le_size by auto.
+realize eq1_size by auto.
+realize bvgetP by auto.
+
+bind op [bool & W11.t] W11.init "init".
+realize size_1 by auto.
+realize bvinitP.
+move => f.  apply (eq_from_nth false).
++ rewrite size_w2bits (size_flatten' 1). 
+  move => x; rewrite mkseqP /= => Hx;elim Hx.
+  rewrite /bool2bits => /#.
+  rewrite size_mkseq /#.
+
+move => i; rewrite size_w2bits => ?.
+rewrite get_w2bits (nth_flatten false 1).
++ rewrite allP.
+  move => x; rewrite mkseqP /= => Hx;elim Hx.
+  rewrite /bool2bits => /#.
+by rewrite nth_mkseq 1:/# /= /bool2bits initiE 1:/# /=. 
+qed.
 
 (* ----------- BEGIN W12 BINDINGS -----------*)
 
@@ -271,8 +246,30 @@ rewrite -bs2int_mod 1:// /= /to_uint.
 have ?: W12.modulus = 4096 by done.
 by smt(bs2int_range mem_range W12.size_w2bits).
 qed.
+realize gt0_size by done.
+
+bind op [W12.t & bool] W12."_.[_]" "get".
+realize le_size by auto.
+realize eq1_size by auto.
+realize bvgetP by auto.
 
 
+bind op [bool & W12.t] W12.init "init".
+realize size_1 by auto.
+realize bvinitP.
+move => f.  apply (eq_from_nth false).
++ rewrite size_w2bits (size_flatten' 1). 
+  move => x; rewrite mkseqP /= => Hx;elim Hx.
+  rewrite /bool2bits => /#.
+  rewrite size_mkseq /#.
+
+move => i; rewrite size_w2bits => ?.
+rewrite get_w2bits (nth_flatten false 1).
++ rewrite allP.
+  move => x; rewrite mkseqP /= => Hx;elim Hx.
+  rewrite /bool2bits => /#.
+by rewrite nth_mkseq 1:/# /= /bool2bits initiE 1:/# /=.
+qed.
 
 (* ----------- BEGIN W16 BINDINGS ---------- *)
 
@@ -291,9 +288,11 @@ rewrite -bs2int_mod 1:// /= /to_uint.
 by smt(bs2int_range mem_range W16.size_w2bits pow2_16).
 qed.
 realize touintP by smt().
+realize gt0_size by done.
 
 bind op W16.t W16.( + ) "add".
 realize bvaddP by exact W16.to_uintD.
+
 
 bind op W16.t W16.( * ) "mul".
 realize bvmulP by exact W16.to_uintM. 
@@ -304,6 +303,9 @@ realize bvultP by move=> bv1 bv2; rewrite W16.ultE /#.
 
 bind op [bool & W16.t] W16.\slt "slt".
 realize bvsltP by move=> w1 w2; rewrite W16.sltE /#.
+
+bind op [bool & W16.t] W16.\sle "sle".
+realize bvsleP by  move=> w1 w2; rewrite W16.sleE /#. 
 
 bind op W16.t W16.andw "and".
 realize bvandP. 
@@ -374,13 +376,14 @@ by have -> : (2 ^ (8 - i) * 2 ^ i) = 256;
   [ rewrite -StdBigop.Bigint.Num.Domain.exprD_nneg 
      1,2:/# /= -!addrA /= | done ].
 qed.
-
+realize le_size by done.
 
 bind op [W8.t & W16.t] W2u8.zeroextu16 "zextend".
 realize bvzextendP.
 move => bv; rewrite /zeroextu16 /= of_uintK /= modz_small 2://.
 apply bound_abs; smt(W8.to_uint_cmp pow2_8).
 qed.
+realize le_size by done.
 
 op truncateu12(a : W16.t) : W12.t =
     W12.of_int (to_uint a).
@@ -403,6 +406,7 @@ by have -> : (2 ^ (12 - i) * 2 ^ i) = 4096;
   [ rewrite -StdBigop.Bigint.Num.Domain.exprD_nneg 
      1,2:/# /= -!addrA /= | done ].
 qed.
+realize le_size by done.
 
 op zeroextu16(a : W12.t) : W16.t =
     W16.of_int (to_uint a).
@@ -413,36 +417,76 @@ move => bv; rewrite /zeroextu16 /= of_uintK /=.
 have /= := W12.to_uint_cmp.
 by smt().
 qed.
+realize le_size by done.
+
+bind op [bool & W16.t] W16.init "init".
+realize size_1 by auto.
+realize bvinitP.
+move => f.  apply (eq_from_nth false).
++ rewrite size_w2bits (size_flatten' 1). 
+  move => x; rewrite mkseqP /= => Hx;elim Hx.
+  rewrite /bool2bits => /#.
+  rewrite size_mkseq /#.
+
+move => i; rewrite size_w2bits => ?.
+rewrite get_w2bits (nth_flatten false 1).
++ rewrite allP.
+  move => x; rewrite mkseqP /= => Hx;elim Hx.
+  rewrite /bool2bits => /#.
+by rewrite nth_mkseq 1:/# /= /bool2bits initiE 1:/# /=. 
+qed.
 
 (* ----------- BEGIN W20 BINDINGS -----------*)
 
 theory W20.
-  abbrev [-printing] size = 20.
-  clone include BitWordSH with op size <- size
-  rename "_XX" as "_20"
-  proof gt0_size by done, size_le_256 by done.
-end W20.
+abbrev [-printing] size = 20.
+clone include BitWordSH with op size <- size
+rename "_XX" as "_20"
+proof gt0_size by done,
+size_le_256 by done.
 
-import W20.
+end W20. export W20 W20.ALU W20.SHIFT.
 
-(* -------------------------------------------------------------------- *)
+
 bind bitstring W20.w2bits W20.bits2w W20.to_uint W20.to_sint W20.of_int W20.t 20.
 realize size_tolist by auto.
-realize tolistP     by auto.
-realize oflistP     by smt(W20.bits2wK).
-realize ofintP      by move=> *; rewrite /of_int int2bs_mod.
-realize touintP     by smt().
-
-realize tosintP.
-proof.
-move=> bv /= @/to_sint @/smod @/msb.
-rewrite (_ : nth _ _ _ = 2 ^ (20 - 1) <= to_uint bv) -1:/#.
-rewrite /to_uint -{2}(cat_take_drop 11 (w2bits bv)).
+realize tolistP by auto.
+realize oflistP by smt(W20.bits2wK). 
+realize ofintP by move => *;rewrite /of_int int2bs_mod.
+realize tosintP. move => bv /=;rewrite /to_sint /smod /BVA_Top_W20_t.msb.
+have -> /=: nth false (w2bits bv) (20 - 1) = 2 ^ (20 - 1) <= to_uint bv; last by smt().
+rewrite /to_uint. 
+rewrite -{2}(cat_take_drop 10 (w2bits bv)).
 rewrite bs2int_cat size_take 1:// W20.size_w2bits /=.
 rewrite -bs2int_div 1:// /= get_to_uint /=.
 rewrite -bs2int_mod 1:// /= /to_uint.
-have ?: W20.modulus = 1048576 by done.
+have ? : 2^20 = 1048576 by rewrite /=.
 by smt(bs2int_range mem_range W20.size_w2bits).
+qed.
+realize touintP by smt().
+realize gt0_size by done.
+
+
+bind op [W20.t & bool] W20."_.[_]" "get".
+realize le_size by auto.
+realize eq1_size by auto.
+realize bvgetP by auto.
+
+bind op [bool & W20.t] W20.init "init".
+realize size_1 by auto.
+realize bvinitP.
+move => f.  apply (eq_from_nth false).
++ rewrite size_w2bits (size_flatten' 1). 
+  move => x; rewrite mkseqP /= => Hx;elim Hx.
+  rewrite /bool2bits => /#.
+  rewrite size_mkseq /#.
+
+move => i; rewrite size_w2bits => ?.
+rewrite get_w2bits (nth_flatten false 1).
++ rewrite allP.
+  move => x; rewrite mkseqP /= => Hx;elim Hx.
+  rewrite /bool2bits => /#.
+by rewrite nth_mkseq 1:/# /= /bool2bits initiE 1:/# /=. 
 qed.
 
 
@@ -464,42 +508,8 @@ rewrite -bs2int_mod 1:// /= /to_uint.
 by smt(bs2int_range mem_range W32.size_w2bits pow2_32).
 qed.
 realize touintP by smt().
+realize gt0_size by done.
 
-op truncateu_32_20(a : W32.t) : W20.t =
-    W20.of_int (to_uint a).
-
-bind op [W32.t & W20.t] truncateu_32_20 "truncate".
-realize bvtruncateP.
-move => mv; rewrite /truncateu_32_20 /W32.w2bits take_mkseq 1:// /= /w2bits.
-apply (eq_from_nth witness);1: by smt(size_mkseq).
-move => i; rewrite size_mkseq /= /max /= => ib.
-rewrite !nth_mkseq 1..2:// /of_int /to_uint /= get_bits2w 1:// 
-        nth_mkseq 1:// /= get_to_uint 1:// /= /to_uint /=.
-have -> /=: (0 <= i && i < 32) by smt().
-pose a := bs2int (w2bits mv). 
-rewrite {1}(divz_eq a (2^(20-i)*2^i)) !mulrA divzMDl;
-   1: by smt(StdOrder.IntOrder.expr_gt0).
-rewrite dvdz_modzDl; 1: by
- have ->  : 2^(20-i) = 2^((20-i-1)+1); [ by smt() |
-    rewrite exprS 1:/#; smt(dvdz_mull dvdz_mulr)].  
-by have -> : (2 ^ (20 - i) * 2 ^ i) = 1048576; 
-  [ rewrite -StdBigop.Bigint.Num.Domain.exprD_nneg 
-     1,2:/# /= -!addrA /= | done ].
-qed.
-
-op zeroextu_20_32(a : W20.t) : W32.t =
-    W32.of_int (to_uint a).
-
-lemma pow2_20 : 2^20 = 1048576 by auto.
-
-bind op [W20.t & W32.t] zeroextu_20_32 "zextend".
-realize bvzextendP by  move => bv; rewrite /= of_uintK /=; smt(W20.to_uint_cmp pow2_20 pow2_32).
-
-bind op [bool & W32.t] W32.\sle "sle".
-realize bvsleP by move=> bv1 bv2; rewrite W32.sleE /#.
-
-bind op [bool & W32.t] W32.\ule "ule".
-realize bvuleP by move=> bv1 bv2; rewrite W32.uleE /#.
 
 bind op W32.t W32.( + ) "add".
 realize bvaddP by exact W32.to_uintD.
@@ -560,9 +570,11 @@ qed.
 
 bind op [W8.t & W32.t] W4u8.zeroextu32 "zextend".
 realize bvzextendP by move => bv; rewrite /zeroextu32 /= of_uintK /=; smt(W8.to_uint_cmp pow2_8).
+realize le_size by done.
 
 bind op [W16.t & W32.t] W2u16.zeroextu32 "zextend".
 realize bvzextendP by move => bv; rewrite /zeroextu64 /= of_uintK /=; smt(W16.to_uint_cmp pow2_16).
+realize le_size by done.
 
 
 bind op [W16.t & W32.t] sigextu32 "sextend".
@@ -571,6 +583,7 @@ move => bv;rewrite  /sigextu32 /to_sint /smod /= !of_uintK /=.
 case (32768 <= to_uint bv); 2: smt(W16.to_uint_cmp).
 move =>?;rewrite -{2}(oppzK (to_uint bv - 65536)) modNz /=; smt(W16.to_uint_cmp pow2_16). 
 qed.
+realize le_size by done.
 
 bind op [W32.t & W8.t] W4u8.truncateu8 "truncate".
 realize bvtruncateP.
@@ -590,6 +603,7 @@ by have -> : (2 ^ (8 - i) * 2 ^ i) = 256;
   [ rewrite -StdBigop.Bigint.Num.Domain.exprD_nneg 
      1,2:/# /= -!addrA /= | done ].
 qed.
+realize le_size by done.
 
 
 bind op [W32.t & W16.t] W2u16.truncateu16 "truncate".
@@ -610,6 +624,7 @@ by have -> : (2 ^ (16 - i) * 2 ^ i) = 65536;
   [ rewrite -StdBigop.Bigint.Num.Domain.exprD_nneg 
      1,2:/# /= -!addrA /= | done ].
 qed.
+realize le_size by done.
 
 op truncateu32_4(a : W32.t) : W4.t =
     W4.of_int (to_uint a).
@@ -632,12 +647,14 @@ by have -> : (2 ^ (4 - i) * 2 ^ i) = 16;
   [ rewrite -StdBigop.Bigint.Num.Domain.exprD_nneg 
      1,2:/# /= -!addrA /= | done ].
 qed.
+realize le_size by done.
 
 op zeroextu4_32(a : W4.t) : W32.t =
   W32.of_int (to_uint a).
 
 bind op [W4.t & W32.t] zeroextu4_32 "zextend".
 realize bvzextendP by move => bv; rewrite /zeroextu4_32 /= of_uintK /=; smt(W4.to_uint_cmp pow2_4).
+realize le_size by done.
 
 op truncateu32_5(a : W32.t) : W5.t =
     W5.of_int (to_uint a).
@@ -660,12 +677,14 @@ by have -> : (2 ^ (5 - i) * 2 ^ i) = 32;
   [ rewrite -StdBigop.Bigint.Num.Domain.exprD_nneg 
      1,2:/# /= -!addrA /= | done ].
 qed.
+realize le_size by done.
 
 op zeroextu5_32(a : W5.t) : W32.t =
   W32.of_int (to_uint a).
 
 bind op [W5.t & W32.t] zeroextu5_32 "zextend".
 realize bvzextendP by move => bv; rewrite /zeroextu5_32 /= of_uintK /=; smt(W5.to_uint_cmp pow2_5).
+realize le_size by done.
 
 op zeroextu10_32(a : W10.t) : W32.t =
   W32.of_int (to_uint a).
@@ -675,6 +694,7 @@ realize bvzextendP.
 have ? : 2^10 = 1024 by auto.
  by move => bv; rewrite /zeroextu32 /= of_uintK /=; smt(W10.to_uint_cmp).
 qed.
+realize le_size by done.
 
 op zeroextu11_32(a : W11.t) : W32.t =
   W32.of_int (to_uint a).
@@ -684,54 +704,63 @@ realize bvzextendP.
 have ? : 2^11 = 2048 by auto.
  by move => bv; rewrite /zeroextu32 /= of_uintK /=; smt(W11.to_uint_cmp).
 qed.
-
-op truncateu_32_11(a : W32.t) : W11.t =
-    W11.of_int (to_uint a).
-
-bind op [W32.t & W11.t] truncateu_32_11 "truncate".
-realize bvtruncateP.
-move => mv; rewrite /truncateu_32_11 /W32.w2bits take_mkseq 1:// /= /w2bits.
-apply (eq_from_nth witness);1: by smt(size_mkseq).
-move => i; rewrite size_mkseq /= /max /= => ib.
-rewrite !nth_mkseq 1..2:// /of_int /to_uint /= get_bits2w 1:// 
-        nth_mkseq 1:// /= get_to_uint 1:// /= /to_uint /=.
-have -> /=: (0 <= i && i < 32) by smt().
-pose a := bs2int (w2bits mv). 
-rewrite {1}(divz_eq a (2^(11-i)*2^i)) !mulrA divzMDl;
-   1: by smt(StdOrder.IntOrder.expr_gt0).
-rewrite dvdz_modzDl; 1: by
- have ->  : 2^(11-i) = 2^((11-i-1)+1); [ by smt() |
-    rewrite exprS 1:/#; smt(dvdz_mull dvdz_mulr)].  
-by have -> : (2 ^ (11 - i) * 2 ^ i) = 2048; 
-  [ rewrite -StdBigop.Bigint.Num.Domain.exprD_nneg 
-     1,2:/# /= -!addrA /= | done ].
-qed.
-
-op truncateu_32_10(a : W32.t) : W10.t =
-    W10.of_int (to_uint a).
-
-bind op [W32.t & W10.t] truncateu_32_10 "truncate".
-realize bvtruncateP.
-move => mv; rewrite /truncateu_32_10 /W32.w2bits take_mkseq 1:// /= /w2bits.
-apply (eq_from_nth witness);1: by smt(size_mkseq).
-move => i; rewrite size_mkseq /= /max /= => ib.
-rewrite !nth_mkseq 1..2:// /of_int /to_uint /= get_bits2w 1:// 
-        nth_mkseq 1:// /= get_to_uint 1:// /= /to_uint /=.
-have -> /=: (0 <= i && i < 32) by smt().
-pose a := bs2int (w2bits mv). 
-rewrite {1}(divz_eq a (2^(10-i)*2^i)) !mulrA divzMDl;
-   1: by smt(StdOrder.IntOrder.expr_gt0).
-rewrite dvdz_modzDl; 1: by
- have ->  : 2^(10-i) = 2^((10-i-1)+1); [ by smt() |
-    rewrite exprS 1:/#; smt(dvdz_mull dvdz_mulr)].  
-by have -> : (2 ^ (10 - i) * 2 ^ i) = 1024; 
-  [ rewrite -StdBigop.Bigint.Num.Domain.exprD_nneg 
-     1,2:/# /= -!addrA /= | done ].
-qed.
+realize le_size by done.
 
 
 bind op [W32.t & bool] W32."_.[_]" "get".
 realize bvgetP by rewrite /bool2bits.
+realize le_size by done.
+realize eq1_size by done.
+
+bind op [bool & W32.t] W32.init "init".
+realize size_1 by auto.
+realize bvinitP.
+move => f.  apply (eq_from_nth false).
++ rewrite size_w2bits (size_flatten' 1). 
+  move => x; rewrite mkseqP /= => Hx;elim Hx.
+  rewrite /bool2bits => /#.
+  rewrite size_mkseq /#.
+
+move => i; rewrite size_w2bits => ?.
+rewrite get_w2bits (nth_flatten false 1).
++ rewrite allP.
+  move => x; rewrite mkseqP /= => Hx;elim Hx.
+  rewrite /bool2bits => /#.
+by rewrite nth_mkseq 1:/# /= /bool2bits initiE 1:/# /=. 
+qed.
+
+op truncateu_32_20(x : W32.t) : W20.t = W20.of_int (to_uint x).
+bind op [W32.t & W20.t] truncateu_32_20 "truncate".
+realize bvtruncateP.
+move => mv; rewrite /truncateu_32_20 /W32.w2bits take_mkseq 1:// /= /w2bits.
+apply (eq_from_nth witness);1: by smt(size_mkseq).
+move => i; rewrite size_mkseq /= /max /= => ib.
+rewrite !nth_mkseq 1..2:// /of_int /to_uint /= get_bits2w 1:// 
+        nth_mkseq 1:// /= get_to_uint 1:// /= /to_uint /=.
+have -> /=: (0 <= i && i < 32) by smt().
+pose a := bs2int (w2bits mv). 
+rewrite {1}(divz_eq a (2^(20-i)*2^i)) !mulrA divzMDl;
+   1: by smt(StdOrder.IntOrder.expr_gt0).
+rewrite dvdz_modzDl; 1: by
+ have ->  : 2^(20-i) = 2^((20-i-1)+1); [ by smt() |
+    rewrite exprS 1:/#; smt(dvdz_mull dvdz_mulr)].  
+by have -> : (2 ^ (20 - i) * 2 ^ i) = 1048576; 
+  [ rewrite -StdBigop.Bigint.Num.Domain.exprD_nneg 
+     1,2:/# /= -!addrA /= | done ].
+qed.
+realize le_size by done.
+
+op zeroextu_20_32(a : W20.t) : W32.t =
+    W32.of_int (to_uint a).
+
+bind op [W20.t & W32.t] zeroextu_20_32 "zextend".
+realize bvzextendP.
+move => bv; rewrite /zeroextu16 /= of_uintK /=.
+have /= := W20.to_uint_cmp.
+by smt().
+qed.
+realize le_size by done.
+
 
 (* ----------- BEGIN W64 BINDINGS ---------- *)
 
@@ -750,6 +779,7 @@ rewrite -bs2int_mod 1:// /= /to_uint.
 by smt(bs2int_range mem_range W64.size_w2bits pow2_64).
 qed.
 realize touintP by smt().
+realize gt0_size by done.
 
 bind op [bool & W64.t] W64.init "init".
 realize bvinitP.
@@ -764,9 +794,12 @@ rewrite get_w2bits (BitEncoding.BitChunking.nth_flatten false 1 _).
  exact BVA_Top_Pervasive_bool.size_tolist.
 by rewrite (:i %% 1 = 0) 1:/# nth_mkseq 1:/# /bool2bits initiE /=.
 qed.
+realize size_1 by done.
 
 bind op [W64.t & bool] W64."_.[_]" "get".
 realize bvgetP by rewrite /bool2bits.
+realize le_size by done.
+realize eq1_size by done.
 
 bind op W64.t W64.( + ) "add".
 realize bvaddP by exact W64.to_uintD.
@@ -840,14 +873,17 @@ qed.
 bind op [W8.t & W64.t] W8u8.zeroextu64 "zextend".
 realize bvzextendP
  by move => bv; rewrite /zeroextu64 /= of_uintK /=; smt(W8.to_uint_cmp pow2_8).
+realize le_size by done.
 
 bind op [W16.t & W64.t] W4u16.zeroextu64 "zextend".
 realize bvzextendP
  by move => bv; rewrite /zeroextu64 /= of_uintK /=; smt(W16.to_uint_cmp pow2_16).
+realize le_size by done.
 
 bind op [W32.t & W64.t] W2u32.zeroextu64 "zextend".
 realize bvzextendP
  by move => bv; rewrite /zeroextu64 /= of_uintK /=; smt(W32.to_uint_cmp pow2_32).
+realize le_size by done.
 
 bind op [W64.t & W16.t] W4u16.truncateu16 "truncate".
 realize bvtruncateP.
@@ -867,6 +903,7 @@ by have -> : (2 ^ (16 - i) * 2 ^ i) = 65536;
   [ rewrite -StdBigop.Bigint.Num.Domain.exprD_nneg 
      1,2:/# /= -!addrA /= | done ].
 qed.
+realize le_size by done.
 
 op truncate64_10 (bw: W64.t) : W10.t = W10.of_int (W64.to_uint bw).
 
@@ -888,6 +925,7 @@ by have -> : (2 ^ (10 - i) * 2 ^ i) = 1024;
   [ rewrite -StdBigop.Bigint.Num.Domain.exprD_nneg 
      1,2:/# /= -!addrA /= | done ].
 qed.
+realize le_size by done.
 
 op truncate64_11 (bw: W64.t) : W11.t = W11.of_int (W64.to_uint bw).
 
@@ -909,6 +947,7 @@ by have -> : (2 ^ (11 - i) * 2 ^ i) = 2048;
   [ rewrite -StdBigop.Bigint.Num.Domain.exprD_nneg 
      1,2:/# /= -!addrA /= | done ].
 qed.
+realize le_size by done.
 
 bind op [W64.t & W8.t] W8u8.truncateu8 "truncate".
 realize bvtruncateP.  (* generalize *)
@@ -928,6 +967,7 @@ by have -> : (2 ^ (8 - i) * 2 ^ i) = 256;
   [ rewrite -StdBigop.Bigint.Num.Domain.exprD_nneg 
      1,2:/# /= -!addrA /= | done ].
 qed.
+realize le_size by done.
 
 
 
@@ -948,9 +988,11 @@ rewrite -bs2int_mod 1:// /= /to_uint.
 by smt(bs2int_range mem_range W128.size_w2bits pow2_128).
 qed.
 realize touintP by smt().
+realize gt0_size by done.
 
 bind op [W64.t & W128.t] W2u64.zeroextu128 "zextend".
 realize bvzextendP by move => bv; rewrite /zeroextu128 /= of_uintK /=; smt(W64.to_uint_cmp pow2_64).
+realize le_size by done.
 
 bind op [W128.t & W64.t] W2u64.truncateu64 "truncate".
 realize bvtruncateP.
@@ -970,6 +1012,7 @@ by have -> : (2 ^ (64 - i) * 2 ^ i) = 18446744073709551616;
   [ rewrite -StdBigop.Bigint.Num.Domain.exprD_nneg 
      1,2:/# /= -!addrA /= | done ].
 qed.
+realize le_size by done.
 
 bind op [W128.t & W32.t] W4u32.truncateu32 "truncate".
 realize bvtruncateP.
@@ -989,6 +1032,7 @@ by have -> : (2 ^ (32 - i) * 2 ^ i) = 4294967296;
   [ rewrite -StdBigop.Bigint.Num.Domain.exprD_nneg 
      1,2:/# /= -!addrA /= | done ].
 qed.
+realize le_size by done.
 
 (* ----------- BEGIN W256 BINDINGS ---------- *)
 
@@ -1007,6 +1051,7 @@ rewrite -bs2int_mod 1:// /= /to_uint.
 by smt(bs2int_range mem_range W256.size_w2bits pow2_256).
 qed.
 realize touintP by smt().
+realize gt0_size by done.
 
 bind op [bool & W256.t] W256.init "init".
 realize bvinitP.
@@ -1021,9 +1066,12 @@ rewrite get_w2bits (BitEncoding.BitChunking.nth_flatten false 1 _).
  exact BVA_Top_Pervasive_bool.size_tolist.
 by rewrite (:i %% 1 = 0) 1:/# nth_mkseq 1:/# /bool2bits initiE /=.
 qed.
+realize size_1 by done.
 
 bind op [W256.t & bool] W256."_.[_]" "get".
 realize bvgetP by rewrite /bool2bits.
+realize le_size by done.
+realize eq1_size by done.
 
 bind op W256.t W256.andw "and".
 realize bvandP. 
@@ -1079,6 +1127,7 @@ by have -> : (2 ^ (128 - i) * 2 ^ i) = 340282366920938463463374607431768211456;
   [ rewrite -StdBigop.Bigint.Num.Domain.exprD_nneg 
      1,2:/# /= -!addrA /= | done ].
 qed.
+realize le_size by done.
 
 
 (* ----------- BEGIN ARRAY BINDINGS ---------- *)
@@ -1088,165 +1137,220 @@ realize tolistP by done.
 realize get_setP by smt(Array256.get_setE). 
 realize eqP by smt(Array256.tP).
 realize get_out by smt(Array256.get_out).
+realize gt0_size by done.
 
-bind array Array640."_.[_]" Array640."_.[_<-_]" Array640.to_list Array640.of_list Array640.t 640.
-realize tolistP by done.
-realize get_setP by smt(Array640.get_setE). 
-realize eqP by smt(Array640.tP).
-realize get_out by smt(Array640.get_out).
-
-bind array Array320."_.[_]" Array320."_.[_<-_]" Array320.to_list Array320.of_list Array320.t 320.
-realize tolistP by done.
-realize get_setP by smt(Array320.get_setE). 
-realize eqP by smt(Array320.tP).
-realize get_out by smt(Array320.get_out).
-
-(* 
 bind array Array384."_.[_]" Array384."_.[_<-_]" Array384.to_list Array384.of_list Array384.t 384.
 realize tolistP by done.
 realize get_setP by smt(Array384.get_setE). 
 realize eqP by smt(Array384.tP).
 realize get_out by smt(Array384.get_out).
-
+realize gt0_size by done.
 
 bind array Array768."_.[_]" Array768."_.[_<-_]" Array768.to_list Array768.of_list Array768.t 768.
 realize tolistP by done.
 realize get_setP by smt(Array768.get_setE). 
 realize eqP by smt(Array768.tP).
 realize get_out by smt(Array768.get_out).
+realize gt0_size by done.
 
 bind array Array1024."_.[_]" Array1024."_.[_<-_]" Array1024.to_list Array1024.of_list Array1024.t 1024.
 realize tolistP by done.
 realize get_setP by smt(Array1024.get_setE). 
 realize eqP by smt(Array1024.tP).
 realize get_out by smt(Array1024.get_out).
+realize gt0_size by done.
 
 bind array Array1088."_.[_]" Array1088."_.[_<-_]" Array1088.to_list Array1088.of_list Array1088.t 1088.
 realize tolistP by done.
 realize get_setP by smt(Array1088.get_setE). 
 realize eqP by smt(Array1088.tP).
 realize get_out by smt(Array1088.get_out).
+realize gt0_size by done.
 
 bind array Array1152."_.[_]" Array1152."_.[_<-_]" Array1152.to_list Array1152.of_list Array1152.t 1152.
 realize tolistP by done.
 realize get_setP by smt(Array1152.get_setE). 
 realize eqP by smt(Array1152.tP).
 realize get_out by smt(Array1152.get_out).
+realize gt0_size by done.
 
 bind array Array1408."_.[_]" Array1408."_.[_<-_]" Array1408.to_list Array1408.of_list Array1408.t 1408.
 realize tolistP by done.
 realize get_setP by smt(Array1408.get_setE). 
 realize eqP by smt(Array1408.tP).
 realize get_out by smt(Array1408.get_out).
+realize gt0_size by done.
 
 bind array Array1536."_.[_]" Array1536."_.[_<-_]" Array1536.to_list Array1536.of_list Array1536.t 1536.
 realize tolistP by done.
 realize get_setP by smt(Array1536.get_setE). 
 realize eqP by smt(Array1536.tP).
 realize get_out by smt(Array1536.get_out).
+realize gt0_size by done.
 
 bind array Array1568."_.[_]" Array1568."_.[_<-_]" Array1568.to_list Array1568.of_list Array1568.t 1568.
 realize tolistP by done.
 realize get_setP by smt(Array1568.get_setE). 
 realize eqP by smt(Array1568.tP).
 realize get_out by smt(Array1568.get_out).
+realize gt0_size by done.
 
 bind array Array32."_.[_]" Array32."_.[_<-_]" Array32.to_list Array32.of_list Array32.t 32.
 realize tolistP by done.
 realize get_setP by smt(Array32.get_setE). 
 realize eqP by smt(Array32.tP).
 realize get_out by smt(Array32.get_out).
+realize gt0_size by done.
 
 bind array Array16."_.[_]" Array16."_.[_<-_]" Array16.to_list Array16.of_list Array16.t 16.
 realize tolistP by done.
 realize get_setP by smt(Array16.get_setE). 
 realize eqP by smt(Array16.tP).
 realize get_out by smt(Array16.get_out).
+realize gt0_size by done.
 
 bind array Array48."_.[_]" Array48."_.[_<-_]" Array48.to_list Array48.of_list Array48.t 48.
 realize tolistP by done.
 realize get_setP by smt(Array48.get_setE). 
 realize eqP by smt(Array48.tP).
 realize get_out by smt(Array48.get_out).
+realize gt0_size by done.
 
 bind array Array128."_.[_]" Array128."_.[_<-_]" Array128.to_list Array128.of_list Array128.t 128.
 realize tolistP by done.
 realize get_setP by smt(Array128.get_setE). 
 realize eqP by smt(Array128.tP).
 realize get_out by smt(Array128.get_out).
+realize gt0_size by done.
 
 bind array Array160."_.[_]" Array160."_.[_<-_]" Array160.to_list Array160.of_list Array160.t 160.
 realize tolistP by done.
 realize get_setP by smt(Array160.get_setE). 
 realize eqP by smt(Array160.tP).
 realize get_out by smt(Array160.get_out).
+realize gt0_size by done.
 
 bind array Array960."_.[_]" Array960."_.[_<-_]" Array960.to_list Array960.of_list Array960.t 960.
 realize tolistP by done.
 realize get_setP by smt(Array960.get_setE). 
 realize eqP by smt(Array960.tP).
 realize get_out by smt(Array960.get_out).
+realize gt0_size by done.
 
 bind array Array1410."_.[_]" Array1410."_.[_<-_]" Array1410.to_list Array1410.of_list Array1410.t 1410.
 realize tolistP by done.
 realize get_setP by smt(Array1410.get_setE). 
 realize eqP by smt(Array1410.tP).
 realize get_out by smt(Array1410.get_out).
+realize gt0_size by done.
 
 bind array Array4."_.[_]" Array4."_.[_<-_]" Array4.to_list Array4.of_list Array4.t 4.
 realize tolistP by done.
 realize get_setP by smt(Array4.get_setE). 
 realize eqP by smt(Array4.tP).
 realize get_out by smt(Array4.get_out).
+realize gt0_size by done.
 
 bind array Array1."_.[_]" Array1."_.[_<-_]" Array1.to_list Array1.of_list Array1.t 1.
 realize tolistP by done.
 realize get_setP by smt(Array1.get_setE). 
 realize eqP by smt(Array1.tP).
 realize get_out by smt(Array1.get_out).
+realize gt0_size by done.
 
 bind array Array2."_.[_]" Array2."_.[_<-_]" Array2.to_list Array2.of_list Array2.t 2.
 realize tolistP by done.
 realize get_setP by smt(Array2.get_setE). 
 realize eqP by smt(Array2.tP).
 realize get_out by smt(Array2.get_out).
-
+realize gt0_size by done.
 
 bind array Array5."_.[_]" Array5."_.[_<-_]" Array5.to_list Array5.of_list Array5.t 5.
 realize tolistP by done.
 realize get_setP by smt(Array5.get_setE). 
 realize eqP by smt(Array5.tP).
 realize get_out by smt(Array5.get_out).
+realize gt0_size by done.
 
 bind array Array6."_.[_]" Array6."_.[_<-_]" Array6.to_list Array6.of_list Array6.t 6.
 realize tolistP by done.
 realize get_setP by smt(Array6.get_setE). 
 realize eqP by smt(Array6.tP).
 realize get_out by smt(Array6.get_out).
+realize gt0_size by done.
 
 bind array Array7."_.[_]" Array7."_.[_<-_]" Array7.to_list Array7.of_list Array7.t 7.
 realize tolistP by done.
 realize get_setP by smt(Array7.get_setE). 
 realize eqP by smt(Array7.tP).
 realize get_out by smt(Array7.get_out).
+realize gt0_size by done.
 
 bind array Array8."_.[_]" Array8."_.[_<-_]" Array8.to_list Array8.of_list Array8.t 8.
 realize tolistP by done.
 realize get_setP by smt(Array8.get_setE). 
 realize eqP by smt(Array8.tP).
 realize get_out by smt(Array8.get_out).
+realize gt0_size by done.
 
 bind array Array24."_.[_]" Array24."_.[_<-_]" Array24.to_list Array24.of_list Array24.t 24.
 realize tolistP by done.
 realize get_setP by smt(Array24.get_setE). 
 realize eqP by smt(Array24.tP).
 realize get_out by smt(Array24.get_out).
+realize gt0_size by done.
 
 bind array Array25."_.[_]" Array25."_.[_<-_]" Array25.to_list Array25.of_list Array25.t 25.
 realize tolistP by done.
 realize get_setP by smt(Array25.get_setE). 
 realize eqP by smt(Array25.tP).
 realize get_out by smt(Array25.get_out).
+realize gt0_size by done.
+
+bind array Array640."_.[_]" Array640."_.[_<-_]" Array640.to_list Array640.of_list Array640.t 640.
+realize tolistP by done.
+realize get_setP by smt(Array640.get_setE). 
+realize eqP by smt(Array640.tP).
+realize get_out by smt(Array640.get_out).
+realize gt0_size by done.
+
+
+op init_array640_w8(f : int -> W8.t) = Array640.init f.
+bind op [W8.t & Array640.t] init_array640_w8 "ainit".
+realize bvainitP.
+proof.
+rewrite /init_array640_w8 => f.
+rewrite BVA_Top_Array640_Array640_t.tolistP.
+apply eq_in_mkseq => i i_bnd;
+smt(Array640.initE).
+qed.
+
+op init_array24_w8(f : int -> W8.t) = Array24.init f.
+bind op [W8.t & Array24.t] init_array24_w8 "ainit".
+realize bvainitP.
+rewrite /init_array26_w8 => f.
+rewrite BVA_Top_Array24_Array24_t.tolistP.
+apply eq_in_mkseq => i i_bnd;
+smt(Array24.initE).
+qed.
+
+op init_array32_w16(f : int -> W16.t) = Array32.init f.
+bind op [W16.t & Array32.t] init_array32_w16 "ainit".
+realize bvainitP.
+rewrite /init_array32_w16 => f.
+rewrite BVA_Top_Array32_Array32_t.tolistP.
+apply eq_in_mkseq => i i_bnd;
+smt(Array32.initE).
+qed.
+
+op init_array48_w8(f : int -> W8.t) = Array48.init f.
+bind op [W8.t & Array48.t] init_array48_w8 "ainit".
+realize bvainitP.
+rewrite /init_array48_w8 => f.
+rewrite BVA_Top_Array48_Array48_t.tolistP.
+apply eq_in_mkseq => i i_bnd;
+smt(Array48.initE).
+qed.
 
 op init_32_8 (f: int -> W8.t) : W8.t Array32.t = Array32.init f.
 
@@ -1257,6 +1361,24 @@ rewrite /init_32_8 => f.
 rewrite BVA_Top_Array32_Array32_t.tolistP.
 apply eq_in_mkseq => i i_bnd;
 smt(Array32.initE).
+qed.
+
+op init_1088_8(f : int -> W8.t) = Array1088.init f.
+bind op [W8.t & Array1088.t] init_1088_8 "ainit".
+realize bvainitP.
+rewrite /init_1088_8 => f.
+rewrite BVA_Top_Array1088_Array1088_t.tolistP.
+apply eq_in_mkseq => i i_bnd;
+smt(Array1088.initE).
+qed.
+
+op init_768_10(f : int -> W10.t) = Array768.init f.
+bind op [W10.t & Array768.t] init_768_10 "ainit".
+realize bvainitP.
+rewrite /init_768_10 => f.
+rewrite BVA_Top_Array768_Array768_t.tolistP.
+apply eq_in_mkseq => i i_bnd;
+smt(Array768.initE).
 qed.
 
 op init_1568_8 (f: int -> W8.t) : W8.t Array1568.t = Array1568.init f.
@@ -1369,6 +1491,28 @@ apply eq_in_mkseq => i i_bnd;
 smt(Array256.initE).
 qed.
 
+op init_256_32 (f: int -> W32.t) : W32.t Array256.t = Array256.init f.
+
+bind op [W32.t & Array256.t] init_256_32 "ainit".
+realize bvainitP.
+proof.
+rewrite /init_256_32 => f.
+rewrite BVA_Top_Array256_Array256_t.tolistP.
+apply eq_in_mkseq => i i_bnd;
+smt(Array256.initE).
+qed.
+
+op init_256_20 (f: int -> W20.t) : W20.t Array256.t = Array256.init f.
+
+bind op [W20.t & Array256.t] init_256_20 "ainit".
+realize bvainitP.
+proof.
+rewrite /init_256_20 => f.
+rewrite BVA_Top_Array256_Array256_t.tolistP.
+apply eq_in_mkseq => i i_bnd;
+smt(Array256.initE).
+qed.
+
 op init_768_16 (f: int -> W16.t) : W16.t Array768.t = Array768.init f.
 
 bind op [W16.t & Array768.t] init_768_16 "ainit".
@@ -1470,6 +1614,50 @@ rewrite BVA_Top_Array1408_Array1408_t.tolistP.
 apply eq_in_mkseq => i i_bnd; smt(Array1408.initE).
 qed.
 
+op init_256_12 (f: int -> W12.t) : W12.t Array256.t = 
+  Array256.init f.
+
+bind op [W12.t & Array256.t] init_256_12 "ainit".
+realize bvainitP.
+rewrite /init_256_12 => f.
+rewrite BVA_Top_Array256_Array256_t.tolistP.
+apply eq_in_mkseq => i i_bnd;
+smt(Array256.initE).
+qed.
+
+op init_1024_12 (f: int -> W12.t) : W12.t Array1024.t = 
+  Array1024.init f.
+
+bind op [W12.t & Array1024.t] init_1024_12 "ainit".
+realize bvainitP.
+rewrite /init_1024_12 => f.
+rewrite BVA_Top_Array1024_Array1024_t.tolistP.
+apply eq_in_mkseq => i i_bnd;
+smt(Array1024.initE).
+qed.
+
+
+op init_768_12 (f: int -> W12.t) : W12.t Array768.t = 
+  Array768.init f.
+
+bind op [W12.t & Array768.t] init_768_12 "ainit".
+realize bvainitP.
+rewrite /init_768_12 => f.
+rewrite BVA_Top_Array768_Array768_t.tolistP.
+apply eq_in_mkseq => i i_bnd;
+smt(Array768.initE).
+qed.
+
+op init_1024_11 (f: int -> W11.t) : W11.t Array1024.t = Array1024.init f.
+
+bind op [W11.t & Array1024.t] init_1024_11 "ainit".
+realize bvainitP.
+rewrite /init_1024_11 => f.
+rewrite BVA_Top_Array1024_Array1024_t.tolistP.
+apply eq_in_mkseq => i i_bnd;
+smt(Array1024.initE).
+qed.
+
 op sliceget8_32_256 (arr: W32.t Array8.t) (offset: int) : W256.t = 
    if 8 %| offset then 
     get256_direct ((init32 (fun (i_0 : int) => arr.[i_0])))%WArray32 (offset %/ 8)
@@ -1486,6 +1674,7 @@ rewrite (BitEncoding.BitChunking.nth_flatten false 32 _).
 rewrite (nth_map W32.zero []); 1: smt(Array8.size_to_list).
 rewrite nth_mkseq 1:/# /(\bits8) initiE 1:/# /= /#.
 qed.
+realize le_size by done.
 
 op sliceget4_64_256 (arr: W64.t Array4.t) (offset: int) : W256.t = 
    if 8 %| offset then 
@@ -1503,6 +1692,7 @@ rewrite (BitEncoding.BitChunking.nth_flatten false 64 _).
 rewrite (nth_map W64.zero []); 1: smt(Array4.size_to_list).
 rewrite nth_mkseq 1:/# /(\bits8) initiE 1:/# /= /#.
 qed.
+realize le_size by done.
 
 op sliceget4_32_128 (arr: W32.t Array4.t) (offset: int) : W128.t = 
    if 8 %| offset then 
@@ -1520,6 +1710,7 @@ rewrite (BitEncoding.BitChunking.nth_flatten false 32 _).
 rewrite (nth_map W32.zero []); 1: smt(Array4.size_to_list).
 rewrite nth_mkseq 1:/# /(\bits8) initiE 1:/# /= /#.
 qed.
+realize le_size by done.
 
 op sliceget16_8_128 (arr: W8.t Array16.t) (offset: int) : W128.t = 
    if 8 %| offset then 
@@ -1537,6 +1728,7 @@ rewrite (BitEncoding.BitChunking.nth_flatten false 8 _).
 rewrite (nth_map W8.zero []); 1: smt(Array16.size_to_list).
 rewrite nth_mkseq 1:/# /= /#.
 qed.
+realize le_size by done.
 
 op sliceget16_16_256 (arr: W16.t Array16.t) (offset: int) : W256.t = 
    if 8 %| offset then 
@@ -1554,6 +1746,7 @@ rewrite (BitEncoding.BitChunking.nth_flatten false 16 _).
 rewrite (nth_map W16.zero []); 1: smt(Array16.size_to_list).
 rewrite nth_mkseq 1:/# /(\bits8) initiE 1:/# /= /#.
 qed.
+realize le_size by done.
 
 op sliceget1024_16_256 (arr: W16.t Array1024.t) (offset: int) : W256.t = 
    if 8 %| offset then 
@@ -1571,6 +1764,7 @@ rewrite (BitEncoding.BitChunking.nth_flatten false 16 _).
 rewrite (nth_map W16.zero []); 1: smt(Array1024.size_to_list).
 rewrite nth_mkseq 1:/# /(\bits8) initiE 1:/# /= /#.
 qed.
+realize le_size by done.
 
 op sliceget160_8_64 (arr: W8.t Array160.t) (offset: int) : W64.t = 
    if 8 %| offset then 
@@ -1588,6 +1782,7 @@ rewrite (BitEncoding.BitChunking.nth_flatten false 8 _).
 rewrite (nth_map W8.zero []); 1: smt(Array160.size_to_list).
 rewrite nth_mkseq /#.
 qed.
+realize le_size by done.
 
 op sliceget128_8_64 (arr: W8.t Array128.t) (offset: int) : W64.t = 
    if 8 %| offset then 
@@ -1605,6 +1800,7 @@ rewrite (BitEncoding.BitChunking.nth_flatten false 8 _).
 rewrite (nth_map W8.zero []); 1: smt(Array128.size_to_list).
 rewrite nth_mkseq /#.
 qed.
+realize le_size by done.
 
 
 op sliceget160_8_16 (arr: W8.t Array160.t) (offset: int) : W16.t = 
@@ -1623,6 +1819,7 @@ rewrite (BitEncoding.BitChunking.nth_flatten false 8 _).
 rewrite (nth_map W8.zero []); 1: smt(Array160.size_to_list).
 rewrite nth_mkseq /#.
 qed.
+realize le_size by done.
 
 op sliceget128_8_16 (arr: W8.t Array128.t) (offset: int) : W16.t = 
    if 8 %| offset then 
@@ -1640,6 +1837,9 @@ rewrite (BitEncoding.BitChunking.nth_flatten false 8 _).
 rewrite (nth_map W8.zero []); 1: smt(Array128.size_to_list).
 rewrite nth_mkseq /#.
 qed.
+realize le_size by done.
+
+
 
 op sliceget1568_8_256 (arr: W8.t Array1568.t) (offset: int) : W256.t = 
    if 8 %| offset then 
@@ -1657,6 +1857,7 @@ rewrite (BitEncoding.BitChunking.nth_flatten false 8 _).
 rewrite (nth_map W8.zero []); 1: smt(Array1568.size_to_list).
 rewrite nth_mkseq /#.
 qed.
+realize le_size by done.
 
 op sliceget1088_8_256 (arr: W8.t Array1088.t) (offset: int) : W256.t = 
    if 8 %| offset then 
@@ -1674,7 +1875,7 @@ rewrite (BitEncoding.BitChunking.nth_flatten false 8 _).
 rewrite (nth_map W8.zero []); 1: smt(Array1088.size_to_list).
 rewrite nth_mkseq /#.
 qed.
-
+realize le_size by done.
 
 op sliceget256_16_256 (arr: W16.t Array256.t) (offset: int) : W256.t = 
    if 8 %| offset then 
@@ -1692,7 +1893,7 @@ rewrite (BitEncoding.BitChunking.nth_flatten false 16 _).
 rewrite (nth_map W16.zero []); 1: smt(Array256.size_to_list).
 by rewrite nth_mkseq /#.
 qed.
-
+realize le_size by done.
 
 op sliceset256_16_256 (arr: W16.t Array256.t) (offset: int) (bv: W256.t) : W16.t Array256.t =
   if 8 %| offset
@@ -1734,6 +1935,7 @@ rewrite (nth_flatten _ 16); 1: by rewrite allP => i;rewrite mapP => He; elim He;
 rewrite (nth_map W16.zero []); 1: smt(Array256.size_to_list).
 rewrite nth_mkseq 1:/# /= bits8E /= initiE /# /=.
 qed.
+realize le_size by done.
 
 op sliceget32_8_256 (arr: W8.t Array32.t) (offset: int) : W256.t = 
 if 8 %| offset then 
@@ -1751,6 +1953,7 @@ rewrite (BitEncoding.BitChunking.nth_flatten false 8 _).
 rewrite (nth_map W8.zero []); 1: smt(Array32.size_to_list).
 by rewrite nth_mkseq /#.
 qed.
+realize le_size by done.
 
 op sliceset32_8_32 (arr: W8.t Array32.t) (offset: int) (bv: W32.t) : W8.t Array32.t =
   if 8 %| offset
@@ -1765,6 +1968,7 @@ proof.
   rewrite StdBigop.Bigint.sumzE /= StdBigop.Bigint.BIA.big_mapT /(\o) /=. 
   rewrite StdBigop.Bigint.big_constz count_predT /#.
 qed.
+
 
 bind op [W8.t & W32.t & Array32.t] sliceset32_8_32 "asliceset".
 realize bvaslicesetP. 
@@ -1792,6 +1996,7 @@ rewrite (nth_flatten _ 8); 1: by rewrite allP => i;rewrite mapP => He; elim He;s
 rewrite (nth_map W8.zero []); 1: smt(Array32.size_to_list).
 rewrite nth_mkseq 1:/# /= /#. 
 qed.
+realize le_size by done.
 
 op sliceset128_8_256 (arr: W8.t Array128.t) (offset: int) (bv: W256.t) : W8.t Array128.t =
   if 8 %| offset
@@ -1825,7 +2030,7 @@ rewrite (nth_flatten _ 8); 1: by rewrite allP => i;rewrite mapP => He; elim He;s
 rewrite (nth_map W8.zero []); 1: smt(Array128.size_to_list).
 rewrite nth_mkseq 1:/# /= /#. 
 qed.
-
+realize le_size by done.
 
 op sliceset384_8_256 (arr: W8.t Array384.t) (offset: int) (bv: W256.t) : W8.t Array384.t =
   if 8 %| offset
@@ -1859,7 +2064,7 @@ rewrite (nth_flatten _ 8); 1: by rewrite allP => i;rewrite mapP => He; elim He;s
 rewrite (nth_map W8.zero []); 1: smt(Array384.size_to_list).
 rewrite nth_mkseq 1:/# /= /#. 
 qed.
-
+realize le_size by done.
 
 
 op sliceget384_8_256 (arr: W8.t Array384.t) (offset: int) : W256.t = 
@@ -1878,6 +2083,7 @@ rewrite (BitEncoding.BitChunking.nth_flatten false 8 _).
 rewrite (nth_map W8.zero []); 1: smt(Array384.size_to_list).
 by rewrite nth_mkseq /#.
 qed.
+realize le_size by done.
 
 op sliceget768_16_256 (arr: W16.t Array768.t) (offset: int) : W256.t =
 if 8 %| offset then 
@@ -1896,6 +2102,7 @@ rewrite (BitEncoding.BitChunking.nth_flatten false 16 _).
 rewrite (nth_map W16.zero []); 1: smt(Array768.size_to_list).
 by rewrite nth_mkseq /#.
 qed.
+realize le_size by done.
 
 op sliceset960_8_128 (arr: W8.t Array960.t) (offset: int) (bv: W128.t) : W8.t Array960.t = 
   if 8 %| offset
@@ -1929,6 +2136,7 @@ rewrite (nth_flatten _ 8); 1: by rewrite allP => i;rewrite mapP => He; elim He;s
 rewrite (nth_map W8.zero []); 1: smt(Array960.size_to_list).
 rewrite nth_mkseq /#.
 qed.
+realize le_size by done.
 
 op sliceset160_8_128 (arr: W8.t Array160.t) (offset: int) (bv: W128.t) : W8.t Array160.t = 
   if 8 %| offset
@@ -1963,6 +2171,7 @@ rewrite (nth_flatten _ 8); 1: by rewrite allP => i;rewrite mapP => He; elim He;s
 rewrite (nth_map W8.zero []); 1: smt(Array160.size_to_list).
 rewrite nth_mkseq /#.
 qed.
+realize le_size by done.
 
 
 op sliceset160_8_32 (arr: W8.t Array160.t) (offset: int) (bv: W32.t) : W8.t Array160.t = 
@@ -1998,6 +2207,7 @@ rewrite (nth_flatten _ 8); 1: by rewrite allP => i;rewrite mapP => He; elim He;s
 rewrite (nth_map W8.zero []); 1: smt(Array160.size_to_list).
 rewrite nth_mkseq /#.
 qed.
+realize le_size by done.
 
 op sliceset1410_8_128 (arr: W8.t Array1410.t) (offset: int) (bv: W128.t) : W8.t Array1410.t = 
   if 8 %| offset
@@ -2032,6 +2242,7 @@ rewrite (nth_flatten _ 8); 1: by rewrite allP => i;rewrite mapP => He; elim He;s
 rewrite (nth_map W8.zero []); 1: smt(Array1410.size_to_list).
 rewrite nth_mkseq /#.
 qed.
+realize le_size by done.
 
 op sliceset1410_8_64 (arr: W8.t Array1410.t) (offset: int) (bv: W64.t) : W8.t Array1410.t = 
   if 8 %| offset
@@ -2066,6 +2277,7 @@ rewrite (nth_flatten _ 8); 1: by rewrite allP => i;rewrite mapP => He; elim He;s
 rewrite (nth_map W8.zero []); 1: smt(Array1410.size_to_list).
 rewrite nth_mkseq /#.
 qed.
+realize le_size by done.
 
 
 op sliceset960_8_32 (arr: W8.t Array960.t) (offset: int) (bv: W32.t) : W8.t Array960.t = 
@@ -2104,6 +2316,7 @@ rewrite (nth_flatten _ 8); 1: by rewrite allP => i;rewrite mapP => He; elim He;s
 rewrite (nth_map W8.zero []); 1: smt(Array960.size_to_list).
 rewrite nth_mkseq /#.
 qed.
+realize le_size by done.
 
 op sliceset768_16_256 (arr: W16.t Array768.t) (offset: int) (bv: W256.t) : W16.t Array768.t = 
   if 8 %| offset
@@ -2140,6 +2353,7 @@ rewrite (nth_flatten _ 16); 1: by rewrite allP => i;rewrite mapP => He; elim He;
 rewrite (nth_map W16.zero []); 1: smt(Array768.size_to_list).
 rewrite nth_mkseq 1:/# /= /(\bits8) initiE 1:/# /#. 
 qed.
+realize le_size by done.
 
 op sliceset1024_16_256 (arr: W16.t Array1024.t) (offset: int) (bv: W256.t) : W16.t Array1024.t = 
   if 8 %| offset
@@ -2176,7 +2390,7 @@ rewrite (nth_flatten _ 16); 1: by rewrite allP => i;rewrite mapP => He; elim He;
 rewrite (nth_map W16.zero []); 1: smt(Array1024.size_to_list).
 rewrite nth_mkseq 1:/# /= /(\bits8) initiE 1:/# /#. 
 qed.
-
+realize le_size by done.
 op init_4_32 (f: int -> W32.t) : W32.t Array4.t = Array4.init f.
 
 bind op [W32.t & Array4.t] init_4_32 "ainit".
@@ -2188,53 +2402,60 @@ smt(Array4.initE).
 qed.
 
 
+
 (* BEGIN BIND CIRCUITS *)
-bind circuit VPBROADCAST_16u16 "VPBROADCAST_16u16".
-bind circuit VPBROADCAST_8u32 "VPBROADCAST_8u32".
-bind circuit VPBROADCAST_4u64 "VPBROADCAST_4u64".
-bind circuit VPMADDWD_256 "VPMADDWD_16u16".
-bind circuit VPSLLV_8u32 "VPSLLV_8u32".
-bind circuit VPSHUFB_256 "VPSHUFB_256".
-bind circuit VEXTRACTI128 "VEXTRACTI128".
-bind circuit VPBLENDW_128 "VPBLENDW_128".
-bind circuit BLENDV_16u8 "VPBLENDVB_128".
-bind circuit VPEXTR_32 "VEXTRACTI32_256".
-bind circuit W4u32.VPEXTR_32 "VEXTRACTI32_128".
-bind circuit VPMULH_16u16 "VPMULH_16u16".
-bind circuit VPMULHRS_16u16 "VPMULHRS_16u16".
-bind circuit VPMULL_16u16 "VPMULL_16u16".
-bind circuit VPSUB_16u16 "VPSUB_16u16".
-bind circuit VPADD_16u16 "VPADD_16u16".
-bind circuit W32.mulhi "UMULHI_32".
+bind circuit
+    VPBROADCAST_16u16 <- "VPBROADCAST_16u16",
+    VPBROADCAST_8u32 <- "VPBROADCAST_8u32",
+    VPBROADCAST_4u64 <- "VPBROADCAST_4u64",
+    VPMADDWD_256 <- "VPMADDWD_16u16",
+    VPSLLV_8u32 <- "VPSLLV_8u32",
+    VPSHUFB_256 <- "VPSHUFB_256",
+    VEXTRACTI128 <- "VEXTRACTI128",
+    VINSERTI128    <-   "VPINSERTI128",
+    VPBLENDW_128 <- "VPBLENDW_128",
+    BLENDV_16u8 <- "VPBLENDVB_128",
+    VPEXTR_32 <- "VEXTRACTI32_256",
+    W4u32.VPEXTR_32 <- "VEXTRACTI32_128", (* FIXME: WHY ARE WE USING THIS BINDING? *)
+    VPMULH_16u16 <- "VPMULH_16u16",
+    VPMULHRS_16u16 <- "VPMULHRS_16u16",
+    VPMULL_16u16 <- "VPMULL_16u16",
+    VPSUB_16u16 <- "VPSUB_16u16",
+    VPADD_16u16 <- "VPADD_16u16",
+    VPADD_32u8     <-   "VPADD_32u8",
 
-bind circuit VPSHUFD_256 "VPSHUFD_256".
-bind circuit VPERMQ "VPERMQ".
-bind circuit VPERMD "VPERMD".
-bind circuit VPSRL_4u64 "VPSRL_4u64".
-bind circuit VPADD_4u64 "VPADD_4u64".
-bind circuit VPBLENDD_256 "VPBLEND_8u32".
-bind circuit VPSLLV_4u64 "VPSLLV_4u64".
-bind circuit VPSRLV_4u64 "VPSRLV_4u64".
-bind circuit VPSRLDQ_256 "VPSRLDQ_256".
-bind circuit VPSRLV_8u32 "VPSRLV_8u32".
-bind circuit VPSRLV_16u16 "VPSRLV_16u16".
-bind circuit VPSRL_16u16 "VPSRL_16u16".
-bind circuit VPSRA_16u16 "VPSRA_16u16".
-bind circuit VPSLL_16u16 "VPSLL_16u16".
-bind circuit VPSRL_8u32 "VPSRL_8u32".
-bind circuit VPSLL_8u32 "VPSLL_8u32".
-bind circuit VPSLL_4u64 "VPSLL_4u64".
-bind circuit VPINSR_8u16 "VPINSR_8u16".
-bind circuit VPBROADCAST_2u128 "VPBROADCAST_2u128".
-bind circuit VPACKUS_16u16 "VPACKUS_16u16".
-bind circuit VPMADDUBSW_256 "VPMADDUBSW_256".
-bind circuit VPERM2I128 "VPERM2I128".
-bind circuit VPUNPCKL_4u64 "VPUNPCKL_4u64".
-bind circuit VPUNPCKH_4u64 "VPUNPCKH_4u64".
-bind circuit VMOVSLDUP_256 "VMOVSLDUP_256".
-bind circuit VPBLENDW_256 "VPBLENDW_256".
-bind circuit VPACKSS_16u16 "VPACKSS_16u16".
-bind circuit MOVEMASK_32u8 "VPMOVMSKB_u256u32".
+    VPSHUFD_256 <- "VPSHUFD_256",
+    VPERMQ <- "VPERMQ",
+    VPERMD <- "VPERMD",
+    VPSRL_4u64 <- "VPSRL_4u64",
+    VPADD_4u64 <- "VPADD_4u64",
+    VPBLENDD_256 <- "VPBLEND_8u32",
+    VPSLLV_4u64 <- "VPSLLV_4u64",
+    VPSRLV_4u64 <- "VPSRLV_4u64",
+    VPSRLDQ_256 <- "VPSRLDQ_256",
+    VPSRLV_8u32 <- "VPSRLV_8u32",
+    VPSRLV_16u16 <- "VPSRLV_16u16",
+    VPSRL_16u16 <- "VPSRL_16u16",
+    VPSRA_16u16 <- "VPSRA_16u16",
+    VPSLL_16u16 <- "VPSLL_16u16",
+    VPSRL_8u32 <- "VPSRL_8u32",
+    VPSLL_8u32 <- "VPSLL_8u32",
+    VPSLL_4u64 <- "VPSLL_4u64",
+    VPINSR_8u16 <- "VPINSR_8u16",
+    VPBROADCAST_2u128 <- "VPBROADCAST_2u128",
+    VPACKUS_16u16 <- "VPACKUS_16u16",
+    VPMADDUBSW_256 <- "VPMADDUBSW_256",
+    VPERM2I128 <- "VPERM2I128",
+    VPUNPCKL_4u64 <- "VPUNPCKL_4u64",
+    VPUNPCKH_4u64 <- "VPUNPCKH_4u64",
+    VMOVSLDUP_256 <- "VMOVSLDUP_256",
+    VPBLENDW_256 <- "VPBLENDW_256",
+    VPACKSS_16u16 <- "VPACKSS_16u16",
+    MOVEMASK_32u8 <- "VPMOVMSKB_u256u32",
+
+    VPUNPCKL_32u8  <-   "VPUNPCKL_32u8",
+    VPSHUFB_128    <-   "VPSHUFB_128",
+    VPCMPGT_16u16  <-   "VPCMPGT_16u16",
+    VPACKSS_16u16  <-   "VPACKSS_16u16".
 
 
-*)
